Sanitize slice library

examples/lowparse/LowParse.Slice.fst
@@ -18,12 +18,21 @@ type bytes = Seq.seq byte
 type lbuffer (len: nat) = b:B.buffer byte{B.length b == len}
 
 // augment a buffer with a runtime length
-noeq type bslice =
-  | BSlice : len:U32.t -> p:lbuffer (U32.v len) -> bslice
+private
+noeq type bslice_ =
+  | BSlice : len:U32.t -> p:lbuffer (U32.v len) -> bslice_
+
+let bslice = bslice_
 
 inline_for_extraction
 let length (b: bslice) : Tot U32.t = b.len
 let live h (b: bslice) = B.live h b.p
+
+inline_for_extraction
+let as_buffer
+  (b: bslice)
+: Tot (lbuffer (U32.v (length b)))
+= b.p
 
 noextract
 let as_seq h (b: bslice) : Ghost (s:bytes{Seq.length s == U32.v b.len})
@@ -35,33 +44,72 @@ let length_as_seq h (b: bslice) : Lemma
   (ensures (Seq.length (as_seq h b) == UInt32.v (length b)))
 = ()
 
-inline_for_extraction
-let advance_slice (b:bslice) (off:U32.t{U32.v off <= U32.v b.len}) : Tot bslice =
+noextract
+let buffer_as_seq_as_buffer (h: HS.mem) (b: bslice) : Lemma
+  (requires (live h b))
+  (ensures (
+    live h b /\
+    B.live h (as_buffer b) /\
+    B.as_seq h (as_buffer b) == as_seq h b
+  ))
+  [SMTPatOr [
+    [SMTPat (B.live h (as_buffer b))];
+    [SMTPat (B.as_seq h (as_buffer b))];
+  ]]
+= ()
+
+let index
+  (b: bslice)
+  (i: U32.t)
+: HST.Stack byte
+  (requires (fun h ->
+    live h b /\
+    U32.v i < U32.v (length b)
+  ))
+  (ensures (fun h v h' ->
+    h' == h /\
+    live h' b /\
+    U32.v i < U32.v (length b) /\
+    v == Seq.index (as_seq h b) (U32.v i)
+  ))
+= B.index b.p i
+
+let advanced_slice (b: bslice) (off:U32.t{U32.v off <= U32.v b.len}) : GTot bslice =
   BSlice (U32.sub b.len off) (B.sub b.p off (U32.sub b.len off))
 
-let advance_slice_spec (b:bslice) (off:U32.t{U32.v off <= U32.v b.len}) h :
+inline_for_extraction
+let advance_slice (b:bslice) (off:U32.t{U32.v off <= U32.v b.len}) : HST.Stack bslice
+  (requires (fun h -> live h b))
+  (ensures (fun h b' h' ->
+    h' == h /\
+    b' == advanced_slice b off
+  ))
+= BSlice (U32.sub b.len off) (B.sub b.p off (U32.sub b.len off))
+
+let advanced_slice_spec (b:bslice) (off:U32.t{U32.v off <= U32.v b.len}) h :
   Lemma (requires (live h b))
-        (ensures (live h (advance_slice b off) /\
-                  as_seq h (advance_slice b off) == Seq.slice (as_seq h b) (U32.v off) (Seq.length (as_seq h b))))
+        (ensures (live h (advanced_slice b off) /\
+		  as_buffer (advanced_slice b off) == B.sub (as_buffer b) off (U32.sub (length b) off) /\
+                  as_seq h (advanced_slice b off) == Seq.slice (as_seq h b) (U32.v off) (Seq.length (as_seq h b))))
   = ()
 
-let advance_slice_advance_slice
+let advanced_slice_advanced_slice
   (b: bslice)
   (off1: U32.t {U32.v off1 <= U32.v (length b) } )
-  (off2: U32.t {U32.v off2 <= U32.v (advance_slice b off1).len } )
+  (off2: U32.t {U32.v off2 <= U32.v (advanced_slice b off1).len } )
 : Lemma
   (requires (
     True
   ))
   (ensures (
-    advance_slice (advance_slice b off1) off2 == advance_slice b (U32.add off1 off2)
+    advanced_slice (advanced_slice b off1) off2 == advanced_slice b (U32.add off1 off2)
   ))
-= let s1 = advance_slice b off1 in
-  let s2 = advance_slice s1 off2 in
+= let s1 = advanced_slice b off1 in
+  let s2 = advanced_slice s1 off2 in
   B.sub_sub (BSlice?.p b) off1 (BSlice?.len s1) off2 (BSlice?.len s2)
 
 // pure version of truncate_slice (which is in Stack)
-val truncated_slice : b:bslice -> len:U32.t{U32.v len <= U32.v b.len} -> Tot bslice
+val truncated_slice : b:bslice -> len:U32.t{U32.v len <= U32.v b.len} -> GTot bslice
 let truncated_slice b len = BSlice len (B.sub b.p (U32.uint_to_t 0) len)
 
 inline_for_extraction
@@ -74,209 +122,22 @@ val truncate_slice : b:bslice -> len:U32.t{U32.v len <= U32.v b.len} -> HST.Stac
                         as_seq h1 r == Seq.slice (as_seq h1 b) 0 (U32.v len)))
 let truncate_slice b len = BSlice len (B.sub b.p (U32.uint_to_t 0) len)
 
+let as_buffer_truncated_slice
+  (b: bslice)
+  (len: U32.t{U32.v len <= U32.v b.len})
+: Lemma
+  (as_buffer (truncated_slice b len) == B.sub (as_buffer b) 0ul len)
+= ()
+
 let includes b b' = B.includes b.p b'.p
 
-let bslice_prefix (b b':bslice) : GTot Type0 =
-    // B.includes b'.p b.p means b'.p is the larger buffer
-    B.includes b'.p b.p /\
-    B.idx b.p + B.length b.p == B.idx b'.p + B.length b'.p
-
-val bslice_prefix_equals (b b': bslice) (h0 h1: HS.mem) :
-    Lemma (requires (live h0 b' /\
-                    live h1 b' /\
-                    as_seq h0 b' == as_seq h1 b' /\
-                    bslice_prefix b b'))
-          (ensures (live h0 b /\
-                    live h1 b /\
-                    as_seq h0 b = as_seq h1 b))
-          [SMTPat (bslice_prefix b b'); SMTPat (as_seq h0 b'); SMTPat (as_seq h1 b')]
-let bslice_prefix_equals b b' h0 h1 =
-    B.includes_as_seq h0 h1 b'.p b.p
-
-let bslice_prefix_trans (x y z: bslice) :
-    Lemma (requires (bslice_prefix x y /\ bslice_prefix y z))
-          (ensures (bslice_prefix x z)) = ()
+let includes_trans (b1 b2 b3: bslice) : Lemma
+  (requires (includes b1 b2 /\ includes b2 b3))
+  (ensures (includes b1 b3))
+= B.includes_trans b1.p b2.p b3.p
 
 (*! Framing slices *)
 
 let modifies_none = B.modifies_none
 
-val modifies_slice : b:bslice -> h: HS.mem -> h': HS.mem -> GTot Type0
-let modifies_slice b h h' =
-  B.modifies_1 b.p h h'
-
-let modifies_prefix (b:bslice) (len:U32.t{U32.v len <= U32.v b.len}) =
-  modifies_slice (truncated_slice b len)
-
-let u32_max (a b:U32.t) : max:U32.t{U32.lte a max /\ U32.lte b max} =
-  if U32.gt a b then a else b
-
-let modifies_prefix_plus (b:bslice) (len1 len2: off:U32.t{U32.v off <= U32.v b.len}) h h' h''
-  : Lemma (requires (modifies_prefix b len1 h h' /\
-                     modifies_prefix b len2 h' h''))
-          (ensures (modifies_prefix b (u32_max len1 len2) h h'')) =
-  B.lemma_reveal_modifies_1 (truncated_slice b len1).p h h';
-  B.lemma_reveal_modifies_1 (truncated_slice b len2).p h' h'';
-  B.lemma_intro_modifies_1 (truncated_slice b (u32_max len1 len2)).p h h'';
-  ()
-
-let modifies_prefix_times (b:bslice) (len1: U32.t) (len2: U32.t{U32.v len1 + U32.v len2 <= U32.v b.len}) h h' h''
-  : Lemma (requires (U32.v len1 + U32.v len2 < pow2 32 /\
-                     modifies_prefix b len1 h h' /\
-                     modifies_prefix (advance_slice b len1) len2 h' h''))
-          (ensures (modifies_prefix b (U32.add len1 len2) h h'')) =
-  B.lemma_reveal_modifies_1 (truncated_slice b len1).p h h';
-  B.lemma_reveal_modifies_1 (truncated_slice (advance_slice b len1) len2).p h' h'';
-  B.lemma_intro_modifies_1 (truncated_slice b (U32.add len1 len2)).p h h'';
-  ()
-
-// similar to B.includes, but no restriction on indices (and thus an
-// equivalence)
-let same_ref (#a:Type) (b1 b2:B.buffer a) =
-    B.frameOf b1 == B.frameOf b2 /\
-    B.max_length b1 == B.max_length b2 /\
-    B.content b1 == B.content b2
-
-// XXX: why is this not in the standard library?
-let same_ref_equivalence (#a:Type) :
-    Lemma ((forall b. same_ref #a b b) /\
-           (forall b1 b2. same_ref #a b1 b2 ==> same_ref b2 b1) /\
-           (forall b1 b2 b3. same_ref #a b1 b2 ==> same_ref b2 b3 ==> same_ref b1 b3)) = ()
-
-// b2 starts exactly after b1 ends (for the same underlying ref)
-let buffers_adjacent (#a:Type) (b1 b2:B.buffer a) : Type0 =
-    same_ref b1 b2 /\
-    B.idx b2 == B.idx b1 + B.length b1
-
-let is_concat_of (#a:Type) (b b1 b2:B.buffer a) : Type0 =
-    same_ref b b1 /\
-    same_ref b b2 /\
-    buffers_adjacent b1 b2 /\
-    B.idx b1 == B.idx b /\
-    B.length b1 + B.length b2 == B.length b
-
-let is_concat_liveness (#a:Type) (b b1 b2:B.buffer a) h :
-    Lemma (requires (is_concat_of b b1 b2 /\ B.live h b))
-          (ensures (B.live h b <==> B.live h b1 /\ B.live h b2)) = ()
-
-let is_concat_disjoint (#a:Type) (b b1 b2:B.buffer a) :
-    Lemma (requires (is_concat_of b b1 b2))
-          (ensures (B.disjoint b1 b2)) = ()
-
-let is_concat_append (#a:Type) (b b1 b2:B.buffer a) h :
-    Lemma (requires (is_concat_of b b1 b2 /\
-                     B.live h b))
-          (ensures (B.live h b /\
-                    B.live h b1 /\
-                    B.live h b2 /\
-                    B.as_seq h b == B.as_seq h b1 `Seq.append` B.as_seq h b2)) =
-    Seq.lemma_eq_intro (B.as_seq h b) (B.as_seq h b1 `Seq.append` B.as_seq h b2)
-
-let is_concat_suffix (#a:Type) (b b1 b2:B.buffer a) h :
-    Lemma (requires (is_concat_of b b1 b2 /\
-                     B.live h b))
-          (ensures (B.live h b /\
-                    B.live h b2 /\
-                    // just to satisfy the bounds in the refinements to slice
-                    B.length b1 + B.length b2 == B.length b /\
-                    B.as_seq h b2 == Seq.slice (B.as_seq h b) (B.length b1) (B.length b))) =
-    Seq.lemma_eq_intro (B.as_seq h b2) (Seq.slice (B.as_seq h b) (B.length b1) (B.length b))
-
-let is_concat_prefix (#a:Type) (b b1 b2:B.buffer a) h :
-    Lemma (requires (is_concat_of b b1 b2 /\
-                     B.live h b))
-          (ensures (B.live h b /\
-                    B.live h b1 /\
-                    // just to satisfy the bounds in the refinements to slice
-                    B.length b1 + B.length b2 == B.length b /\
-                    B.as_seq h b1 == Seq.slice (B.as_seq h b) 0 (B.length b1))) =
-    Seq.lemma_eq_intro (B.as_seq h b1) (Seq.slice (B.as_seq h b) 0 (B.length b1))
-
-(*! Splitting buffers *)
-
-(** This single primitive is sufficient to encode many useful patterns, and
-because it always creates disjoint slices it tends to have much easier framing
-than the general [B.sub]. *)
-
-// general split_at primitive (think of Rust's slice::split_at_mut)
-// polymorphic: inline and hope that it type-checks in kremlin
-[@"substitute"]
-val buffer_split_at: #a:Type -> b:B.buffer a ->
-    off:U32.t{U32.v off <= B.length b} ->
-    // TODO: this shouldn't be necessary, but Buffer provides no way to advance
-    // a pointer without specifying a new length
-    // TODO: the above is wrong, there's B.offset to do exactly what we want for
-    // the second buffer
-    len:U32.t{U32.v len == B.length b} ->
-    Pure (B.buffer a * B.buffer a)
-         (requires True)
-         (ensures (fun r ->
-                     let (b1, b2) = r in
-                     is_concat_of b b1 b2 /\
-                     B.length b1 == U32.v off))
-[@"substitute"]
-let buffer_split_at #a b off len =
-    (B.sub b 0ul off, B.sub b off (U32.sub len off))
-
-val bslice_split_at: b:bslice -> off:U32.t{U32.v off <= U32.v b.len} ->
-    Pure (bslice * bslice)
-         (requires True)
-         (ensures (fun r->
-                     let (b1, b2) = r in
-                     is_concat_of b.p b1.p b2.p /\
-                     b1.len == off /\
-                     U32.v b2.len == U32.v b.len - U32.v off))
-let bslice_split_at b off =
-    let (b1, b2) = buffer_split_at b.p off b.len in
-    (BSlice off b1, BSlice (U32.sub b.len off) b2)
-
-// TODO: this proof is somewhat tricky; it boils down to any buffer disjoint to
-// truncated_slice is either some other underlying storage or a subset of
-// advance_slice, and we've assumed that the advance slices are equal
-val modifies_prefix_seq_intro (b:bslice) (len: U32.t{U32.v len <= U32.v b.len}) (h0 h1: HS.mem) :
-  Lemma (requires (modifies_slice b h0 h1 /\
-                   live h0 b /\
-                   live h1 b /\
-                   begin
-                    let len = U32.v len in
-                    let s0 = as_seq h0 b in
-                    let s1 = as_seq h1 b in
-                    forall (i:nat{len <= i /\ i < U32.v b.len}).{:pattern (Seq.index s0 i); (Seq.index s1 i)}
-                                                                 (Seq.index s0 i == Seq.index s1 i)
-                   end))
-        (ensures (modifies_prefix b len h0 h1))
-let modifies_prefix_seq_intro b len h0 h1 =
-  B.lemma_reveal_modifies_1 b.p h0 h1;
-  admit();
-  B.lemma_intro_modifies_1 (truncated_slice b len).p h0 h1
-
-val modifies_prefix_split (b b1 b2:bslice) (len: U32.t{U32.v len <= U32.v b.len}) (h0 h1: HS.mem) :
-    Lemma (requires (live h0 b /\
-                     live h1 b /\
-                     is_concat_of b.p b1.p b2.p /\
-                     modifies_slice b1 h0 h1))
-          (ensures (is_concat_of b.p b1.p b2.p /\
-                    modifies_prefix b b1.len h0 h1))
-let modifies_prefix_split b b1 b2 len h0 h1 =
-  is_concat_append b.p b1.p b2.p h1;
-  admit();
-  // TODO: this is probably the right proof strategy, but maybe can do a
-  // lower-level proof
-  modifies_prefix_seq_intro b b1.len h0 h1;
-  ()
-
-// modifies_slice b1 ==> modifies_slice (b1+b2)
-let modifies_grow_from_b1 (b b1 b2:bslice) (h0 h1: HS.mem) : Lemma
-    (requires (live h0 b /\ live h1 b /\
-              is_concat_of b.p b1.p b2.p /\
-              modifies_slice b1 h0 h1))
-    (ensures (modifies_slice b h0 h1)) =
-    B.modifies_subbuffer_1 h0 h1 b1.p b.p
-
-// modifies_slice b2 ==> modifies_slice (b1+b2)
-let modifies_grow_from_b2 (b b1 b2:bslice) (h0 h1: HS.mem) : Lemma
-    (requires (live h0 b /\ live h1 b /\
-              is_concat_of b.p b1.p b2.p /\
-              modifies_slice b2 h0 h1))
-    (ensures (modifies_slice b h0 h1)) =
-    B.modifies_subbuffer_1 h0 h1 b2.p b.p
+(*! Splitting slices into two parts *)
